proof/crefine/ARM/IsolatedThreadAction.thy
@@ -5,7 +5,7 @@
  *)
 
 theory IsolatedThreadAction
-imports "CLib.MonadicRewrite_C" Finalise_C CSpace_All SyscallArgs_C
+imports ArchMove_C
 begin
 
 datatype tcb_state_regs = TCBStateRegs "thread_state" "MachineTypes.register \<Rightarrow> machine_word"
@@ -119,7 +119,8 @@ lemmas setEndpoint_obj_at_tcb' = setEndpoint_obj_at'_tcb
 
 lemmas setNotification_tcb = set_ntfn_tcb_obj_at'
 
-context kernel_m begin
+context begin interpretation Arch . (*FIXME: arch_split*)
+
 lemma setObject_modify:
   fixes v :: "'a :: pspace_storable" shows
   "\<lbrakk> obj_at' (P :: 'a \<Rightarrow> bool) p s; updateObject v = updateObject_default v;
@@ -137,8 +138,6 @@ lemma setObject_modify:
   apply (simp add: magnitudeCheck_assert in_monad)
   apply (simp add: simpler_modify_def)
   done
-
-context begin interpretation Arch . (*FIXME: arch_split*)
 
 lemma getObject_return:
   fixes v :: "'a :: pspace_storable" shows
@@ -233,6 +232,8 @@ lemma isolate_thread_actions_asUser:
   apply (case_tac ko, simp)
   done
 
+context begin interpretation Arch . (*FIXME: arch_split*)
+
 lemma setRegister_simple:
   "setRegister r v = (\<lambda>con. ({((), con (r := v))}, False))"
   by (simp add: setRegister_def simpler_modify_def)
@@ -240,6 +241,7 @@ lemma setRegister_simple:
 lemma zipWithM_setRegister_simple:
   "zipWithM_x setRegister rs vs
       = (\<lambda>con. ({((), foldl (\<lambda>con (r, v). con (r := v)) con (zip rs vs))}, False))"
+  supply if_split[split del]
   apply (simp add: zipWithM_x_mapM_x)
   apply (induct ("zip rs vs"))
    apply (simp add: mapM_x_Nil return_def)
@@ -260,6 +262,7 @@ lemma map_to_ctes_partial_overwrite:
   "\<forall>x. tcb_at' (idx x) s \<Longrightarrow>
    map_to_ctes (partial_overwrite idx tsrs (ksPSpace s))
      = ctes_of s"
+  supply if_split[split del]
   apply (rule ext)
   apply (frule dom_partial_overwrite[where tsrs=tsrs])
   apply (simp add: map_to_ctes_def partial_overwrite_def
@@ -609,6 +612,7 @@ lemma page_directory_at_partial_overwrite:
 
 lemma findPDForASID_isolatable:
   "thread_actions_isolatable idx (findPDForASID asid)"
+  supply if_split[split del]
   apply (simp add: findPDForASID_def liftE_bindE liftME_def bindE_assoc
                    case_option_If2 assertE_def liftE_def checkPDAt_def
                    stateAssert_def2
@@ -648,6 +652,7 @@ lemma getHWASID_isolatable:
 
 lemma setVMRoot_isolatable:
   "thread_actions_isolatable idx (setVMRoot t)"
+  supply if_split[split del]
   apply (simp add: setVMRoot_def getThreadVSpaceRoot_def
                    locateSlot_conv getSlotCap_def
                    cap_case_isPageDirectoryCap if_bool_simps
@@ -706,24 +711,17 @@ lemma lookupIPC_inv: "\<lbrace>P\<rbrace> lookupIPCBuffer f t \<lbrace>\<lambda>
 
 lemmas empty_fail_user_getreg = empty_fail_asUser[OF empty_fail_getRegister]
 
-lemma user_getreg_rv:
-  "\<lbrace>obj_at' (\<lambda>tcb. P ((atcbContextGet o tcbArch) tcb r)) t\<rbrace> asUser t (getRegister r) \<lbrace>\<lambda>rv s. P rv\<rbrace>"
-  apply (simp add: asUser_def split_def)
-  apply (wp threadGet_wp)
-  apply (clarsimp simp: obj_at'_def projectKOs getRegister_def in_monad atcbContextGet_def)
-  done
-
 lemma copyMRs_simple:
-  "msglen \<le> of_nat (length ARM_H.msgRegisters) \<longrightarrow>
+  "msglen \<le> of_nat (length msgRegisters) \<longrightarrow>
     copyMRs sender sbuf receiver rbuf msglen
-        = forM_x (take (unat msglen) ARM_H.msgRegisters)
+        = forM_x (take (unat msglen) msgRegisters)
              (\<lambda>r. do v \<leftarrow> asUser sender (getRegister r);
                     asUser receiver (setRegister r v) od)
            >>= (\<lambda>rv. return msglen)"
   apply (clarsimp simp: copyMRs_def mapM_discarded)
   apply (rule bind_cong[OF refl])
-  apply (simp add: length_msgRegisters n_msgRegisters_def min_def
-                   word_le_nat_alt
+  apply (simp add: min_def word_le_nat_alt length_msgRegisters
+                   upto_enum_red fromEnum_def enum_register
             split: option.split)
   apply (simp add: upto_enum_def mapM_Nil)
   done
@@ -732,16 +730,16 @@ lemma doIPCTransfer_simple_rewrite:
   "monadic_rewrite True True
    ((\<lambda>_. msgExtraCaps (messageInfoFromWord msgInfo) = 0
                \<and> msgLength (messageInfoFromWord msgInfo)
-                      \<le> of_nat (length ARM_H.msgRegisters))
+                      \<le> of_nat (length msgRegisters))
       and obj_at' (\<lambda>tcb. tcbFault tcb = None
                \<and> (atcbContextGet o tcbArch) tcb msgInfoRegister = msgInfo) sender)
    (doIPCTransfer sender ep badge grant rcvr)
    (do rv \<leftarrow> mapM_x (\<lambda>r. do v \<leftarrow> asUser sender (getRegister r);
                              asUser rcvr (setRegister r v)
                           od)
-               (take (unat (msgLength (messageInfoFromWord msgInfo))) ARM_H.msgRegisters);
+               (take (unat (msgLength (messageInfoFromWord msgInfo))) msgRegisters);
          y \<leftarrow> setMessageInfo rcvr ((messageInfoFromWord msgInfo) \<lparr>msgCapsUnwrapped := 0\<rparr>);
-         asUser rcvr (setRegister ARM_H.badgeRegister badge)
+         asUser rcvr (setRegister badgeRegister badge)
       od)"
   supply if_cong[cong]
   apply (rule monadic_rewrite_gen_asm)
@@ -875,7 +873,7 @@ lemma oblivious_setVMRoot_schact:
 
 lemma oblivious_switchToThread_schact:
   "oblivious (ksSchedulerAction_update f) (ThreadDecls_H.switchToThread t)"
-  apply (simp add: Thread_H.switchToThread_def ARM_H.switchToThread_def bind_assoc
+  apply (simp add: Thread_H.switchToThread_def switchToThread_def bind_assoc
                    getCurThread_def setCurThread_def threadGet_def liftM_def
                    threadSet_def tcbSchedEnqueue_def unless_when asUser_def
                    getQueue_def setQueue_def storeWordUser_def setRegister_def
@@ -937,8 +935,6 @@ begin
 crunch obj_at_dom[wp]: rescheduleRequired "obj_at' (\<lambda>tcb. P (tcbDomain tcb)) t"
 end
 
-context kernel_m begin
-
 lemma setThreadState_no_sch_change:
   "\<lbrace>\<lambda>s. P (ksSchedulerAction s) \<and> (runnable' st \<or> t \<noteq> ksCurThread s)\<rbrace>
       setThreadState st t
@@ -970,6 +966,8 @@ lemma bind_assoc:
      = do x \<leftarrow> m; y \<leftarrow> f x; g y od"
   by (rule bind_assoc)
 
+context begin interpretation Arch . (*FIXME: arch_split*)
+
 lemma setObject_modify_assert:
   "\<lbrakk> updateObject v = updateObject_default v \<rbrakk>
     \<Longrightarrow> setObject p v = do f \<leftarrow> gets (obj_at' (\<lambda>v'. v = v' \<or> True) p);
@@ -994,6 +992,7 @@ lemma setObject_modify_assert:
 
 lemma setEndpoint_isolatable:
   "thread_actions_isolatable idx (setEndpoint p e)"
+  supply if_split[split del]
   apply (simp add: setEndpoint_def setObject_modify_assert
                    assert_def)
   apply (case_tac "p \<in> range idx")
@@ -1087,6 +1086,7 @@ lemma partial_overwrite_fun_upd2:
 
 lemma setCTE_isolatable:
   "thread_actions_isolatable idx (setCTE p v)"
+  supply if_split[split del]
   apply (simp add: setCTE_assert_modify)
   apply (clarsimp simp: thread_actions_isolatable_def
                         monadic_rewrite_def fun_eq_iff
@@ -1149,7 +1149,7 @@ lemma assert_isolatable:
 
 lemma cteInsert_isolatable:
   "thread_actions_isolatable idx (cteInsert cap src dest)"
-  supply if_cong[cong]
+  supply if_split[split del] if_cong[cong]
   apply (simp add: cteInsert_def updateCap_def updateMDB_def
                    Let_def setUntypedCapAsFull_def)
   apply (intro thread_actions_isolatable_bind[OF _ _ hoare_pre(1)]
@@ -1249,7 +1249,7 @@ lemma threadGet_isolatable:
 
  lemma switchToThread_isolatable:
   "thread_actions_isolatable idx (Arch.switchToThread t)"
-  apply (simp add: ARM_H.switchToThread_def
+  apply (simp add: switchToThread_def
                    storeWordUser_def stateAssert_def2)
   apply (intro thread_actions_isolatable_bind[OF _ _ hoare_pre(1)]
                gets_isolatable setVMRoot_isolatable
@@ -1319,7 +1319,7 @@ lemma tcb_at_KOTCB_upd:
         = tcb_at' p s"
   apply (clarsimp simp: obj_at'_def projectKOs objBits_simps
                  split: if_split)
-  apply (simp add: ps_clear_def)
+  apply (fastforce simp add: ps_clear_def)
   done
 
 definition
@@ -1335,6 +1335,7 @@ lemma copy_register_isolate:
                    asUser dest (setRegister r' (rf v)) od)
            (isolate_thread_actions idx (return ())
                  (copy_register_tsrs x y r r' rf) id)"
+  supply if_split[split del]
   apply (simp add: asUser_def split_def bind_assoc
                    getRegister_def setRegister_def
                    select_f_returns isolate_thread_actions_def
@@ -1479,7 +1480,7 @@ lemmas fastpath_isolate_rewrites
 
 lemma lookupIPCBuffer_isolatable:
   "thread_actions_isolatable idx (lookupIPCBuffer w t)"
-  supply if_cong[cong]
+  supply if_split[split del] if_cong[cong]
   apply (simp add: lookupIPCBuffer_def)
   apply (rule thread_actions_isolatable_bind)
   apply (clarsimp simp: put_tcb_state_regs_tcb_def threadGet_isolatable
@@ -1500,6 +1501,7 @@ lemma setThreadState_rewrite_simple:
      (\<lambda>s. (runnable' st \<or> ksSchedulerAction s \<noteq> ResumeCurrentThread \<or> t \<noteq> ksCurThread s) \<and> tcb_at' t s)
      (setThreadState st t)
      (threadSet (tcbState_update (\<lambda>_. st)) t)"
+  supply if_split[split del]
   apply (simp add: setThreadState_def)
   apply (rule monadic_rewrite_imp)
    apply (rule monadic_rewrite_trans)
