proof/crefine/ARM_HYP/Ipc_C.thy
@@ -1535,13 +1535,6 @@ lemma ccorres_add_getRegister:
   apply fastforce
   done
 
-lemma user_getreg_rv:
-  "\<lbrace>obj_at' (\<lambda>tcb. P ((atcbContextGet o tcbArch) tcb r)) t\<rbrace> asUser t (getRegister r) \<lbrace>\<lambda>rv s. P rv\<rbrace>"
-  apply (simp add: asUser_def split_def)
-  apply (wp threadGet_wp)
-  apply (clarsimp simp: obj_at'_def projectKOs getRegister_def in_monad atcbContextGet_def)
-  done
-
 lemma exceptionMessage_ccorres:
   "n < unat n_exceptionMessage
       \<Longrightarrow> register_from_H (ARM_HYP_H.exceptionMessage ! n)
